finish chapter03

exercises/chapter03-state-machines/exercise02.dfy
@@ -12,55 +12,96 @@
 // example to teach you to set up a state machine model.)
 
 // Define all the relevant state in this datatype.
-// FIXME: fill in here (solution: 8 lines)
- datatype Variables = Variables(tableSize: nat)
- {
-   ghost predicate WellFormed() {
-     && 0 < tableSize
-   }
- }
+// DONE: fill in here (solution: 8 lines)
+datatype Variables = Variables(tableSize:nat,
+                               leftHands: seq<bool>,
+                               rightHands: seq<bool>)
+{
+  ghost predicate WellFormed() {
+    && 1 < tableSize
+    && |leftHands| == |rightHands| == tableSize
+    && forall i:nat | i < tableSize :: !(rightHands[i] && leftHands[rightIndex(tableSize, i)])
+  }
+}
 // END EDIT
 
 ghost predicate Init(v:Variables) {
-  // FIXME: fill in here (solution: 3 lines)
-      true  // Replace me
-  // END EDIT
+  // DONE: fill in here (solution: 3 lines)
+  && v.tableSize > 1
+  && v.leftHands == seq(v.tableSize, i => false)
+  && v.rightHands == seq(v.tableSize, i => false)
+     // END EDIT
 }
 
-// FIXME: fill in here (solution: 11 lines)
- // (optional) Add any helper functions desired here
+// DONE: fill in here (solution: 11 lines)
+ghost function rightIndex(tableSize:nat, idx:nat) : (res:nat)
+  requires tableSize > 1
+  requires 0 <= idx < tableSize
+{
+  (idx + 1) % tableSize
+}
+
+ghost function leftIndex(tableSize:nat, idx:nat) : (res:nat)
+  requires tableSize > 1
+  requires 0 <= idx < tableSize
+  ensures (res + 1) % tableSize == idx
+{
+  if idx == 0 then tableSize - 1 else idx - 1
+}
 // END EDIT
 
 // Philosopher with index philosopherIndex acquires left chopstick
 ghost predicate AcquireLeft(v:Variables, v':Variables, philosopherIndex:nat) {
-  // FIXME: fill in here (solution: 5 lines)
-      true  // Replace me
-  // END EDIT
+  // DONE: fill in here (solution: 5 lines)
+  && v.WellFormed()
+  && philosopherIndex < v.tableSize
+  && !v.leftHands[philosopherIndex]
+  && !v.rightHands[leftIndex(v.tableSize, philosopherIndex)]
+  && v' == Variables(v.tableSize,
+                     v.leftHands[philosopherIndex := true],
+                     v.rightHands)
+     // END EDIT
 }
 
 // Philosopher with index philosopherIndex acquires right chopstick
 ghost predicate AcquireRight(v:Variables, v':Variables, philosopherIndex:nat) {
-  // FIXME: fill in here (solution: 5 lines)
-      true  // Replace me
-  // END EDIT
+  // DONE: fill in here (solution: 5 lines)
+  && v.WellFormed()
+  && philosopherIndex < v.tableSize
+  && !v.rightHands[philosopherIndex]
+  && !v.leftHands[rightIndex(v.tableSize, philosopherIndex)]
+  && v' == Variables(v.tableSize,
+                     v.leftHands,
+                     v.rightHands[philosopherIndex := true])
+     // END EDIT
 }
 
 // Philosopher with index philosopherIndex releases both chopsticks
 ghost predicate ReleaseBoth(v:Variables, v':Variables, philosopherIndex:nat) {
-  // FIXME: fill in here (solution: 5 lines)
-      true  // Replace me
-  // END EDIT
+  // DONE: fill in here (solution: 5 lines)
+  && v.WellFormed()
+  && philosopherIndex < v.tableSize
+  && v.leftHands[philosopherIndex]
+  && v.rightHands[philosopherIndex]
+  && v' == Variables(v.tableSize,
+                     v.leftHands[philosopherIndex := false],
+                     v.rightHands[philosopherIndex := false])
+     // END EDIT
 }
 
 datatype Step =
-    // FIXME: fill in here (solution: 3 lines)
-     Step()  // Replace me
+    // DONE: fill in here (solution: 3 lines)
+  | AcquireLeftStep(idx:nat)
+  | AcquireRightStep(idx:nat)
+  | ReleaseBothStep(idx:nat)
     // END EDIT
 
 ghost predicate NextStep(v:Variables, v':Variables, step: Step) {
   match step
-  // FIXME: fill in here (solution: 3 lines)
-   case Step => false  // Replace me
+  // DONE: fill in here (solution: 3 lines)
+  case AcquireLeftStep(idx) => AcquireLeft(v, v', idx)
+  case AcquireRightStep(idx) => AcquireRight(v, v', idx)
+  case ReleaseBothStep(idx) => ReleaseBoth(v, v', idx)
   // END EDIT
 }
 
@@ -80,9 +121,11 @@ ghost predicate Next(v:Variables, v':Variables) {
 ghost predicate NoSticksAcquired(v: Variables)
   requires v.WellFormed()
 {
-  // FIXME: fill in here (solution: 8 lines)
-          true // Replace me
-  // END EDIT
+  // DONE: fill in here (solution: 8 lines)
+  forall i:nat | i < v.tableSize ::
+    && !v.leftHands[i]
+    && !v.rightHands[i]
+       // END EDIT
 }
 
 // Change this predicate to be true if and only if philosopher
@@ -93,8 +136,8 @@ ghost predicate BothSticksAcquired(v: Variables, philosopherIndex: nat)
   requires philosopherIndex < v.tableSize
   requires v.WellFormed()
 {
-  // FIXME: fill in here (solution: 6 lines)
-      true
+  // DONE: fill in here (solution: 6 lines)
+  v.leftHands[philosopherIndex] && v.rightHands[philosopherIndex]
   // END EDIT
 }
 
@@ -103,8 +146,7 @@ lemma InitProperty(v: Variables, philosopherIndex:nat)
   requires Init(v)
   ensures NoSticksAcquired(v)
 {
-  // FIXME: fill in here (solution: 0 lines)
-   // Add a proof (if needed).
+  // DONE: fill in here (solution: 0 lines)
   // END EDIT
 }
 
@@ -120,6 +162,12 @@ lemma PseudoLiveness(philosopherIndex:nat) returns (behavior:seq<Variables>)
   ensures behavior[|behavior|-1].WellFormed() // precondition for calling BothSticksAcquired
   ensures BothSticksAcquired(behavior[|behavior|-1], philosopherIndex)  // Behavior ultimately achieves acquisition for philosopherIndex
 {
-  // FIXME: fill in here (solution: 6 lines)
+  // DONE: fill in here (solution: 6 lines)
+  var state0 := Variables(3, seq(3, i => false), seq(3, i => false));
+  var state1 := Variables(3, seq(3, i => i == philosopherIndex), seq(3, i => false));
+  var state2 := Variables(3, seq(3, i => i == philosopherIndex), seq(3, i => i == philosopherIndex));
+  behavior := [state0, state1, state2];
+  assert NextStep(state0, state1, AcquireLeftStep(philosopherIndex));
+  assert NextStep(state1, state2, AcquireRightStep(philosopherIndex));
   // END EDIT
 }
