exercises/chapter03-state-machines/exercise03.dfy
@@ -16,34 +16,64 @@
 // The safety property is that no two clients ever hold the lock
 // simultaneously.
 
-// FIXME: fill in here (solution: 13 lines)
-datatype Variables = Variables() {
+// DONE: fill in here (solution: 13 lines)
+datatype Variables = Variables(numClients:nat,
+                               serverHolds:bool,
+                               serverFlags:seq<bool>,
+                               clientHolds:seq<bool>)
+{
   ghost predicate WellFormed() {
-    true
+    |serverFlags| == |clientHolds| == numClients
   }
 }
 // END EDIT
 
-
 ghost predicate Init(v:Variables) {
   && v.WellFormed()
-     // FIXME: fill in here (solution: 3 lines)
-                                         && true  // Replace me
+     // DONE: fill in here (solution: 3 lines)
+  && v.serverHolds == true
+  && v.serverFlags == seq(v.numClients, i => false)
+  && v.clientHolds == seq(v.numClients, i => false)
      // END EDIT
 }
-// FIXME: fill in here (solution: 23 lines)
+
+// DONE: fill in here (solution: 23 lines)
+ghost predicate AcquireLock(v:Variables, v':Variables, clientIndex:nat) {
+  && v.WellFormed()
+  && clientIndex < v.numClients
+  && !v.clientHolds[clientIndex]
+  && v.serverHolds
+  && v' == Variables(v.numClients,
+                     false,
+                     v.serverFlags[clientIndex := true],
+                     v.clientHolds[clientIndex := true])
+}
+
+ghost predicate ReleaseLock(v:Variables, v':Variables, clientIndex:nat) {
+  && v.WellFormed()
+  && clientIndex < v.numClients
+  && v.clientHolds[clientIndex]
+  && v.serverFlags[clientIndex]
+  && v' == Variables(v.numClients,
+                     true,
+                     v.serverFlags[clientIndex := false],
+                     v.clientHolds[clientIndex := false])
+}
 // END EDIT
+
 // Jay-Normal-Form: pack all the nondeterminism into a single object
 // that gets there-exist-ed once.
 datatype Step =
-    // FIXME: fill in here (solution: 2 lines)
-   | SomeStep(somearg: int)   // Replace me
+    // DONE: fill in here (solution: 2 lines)
+  | AcquireLockStep(idx:nat)
+  | ReleaseLockStep(idx:nat)
     // END EDIT
 
 ghost predicate NextStep(v:Variables, v':Variables, step: Step) {
   match step
-  // FIXME: fill in here (solution: 2 lines)
-   case SomeStep(somearg) => false  // Replace me
+  // DONE: fill in here (solution: 2 lines)
+  case AcquireLockStep(idx) => AcquireLock(v, v', idx)
+  case ReleaseLockStep(idx) => ReleaseLock(v, v', idx)
   // END EDIT
 }
 
@@ -60,9 +90,12 @@ ghost predicate Next(v:Variables, v':Variables) {
 // may hold the lock simultaneously. This predicate should capture that
 // idea in terms of the Variables you have defined.
 ghost predicate Safety(v:Variables) {
-  // FIXME: fill in here (solution: 10 lines)
-        false  // Replace me
-  // END EDIT
+  // DONE: fill in here (solution: 10 lines)
+  && v.WellFormed()
+  && (forall c1:nat, c2:nat | c1 < v.numClients && c2 < v.numClients ::
+        v.clientHolds[c1] && v.clientHolds[c2] ==> c1 == c2)
+  && (forall i:nat | i < v.numClients :: v.serverFlags[i] == v.clientHolds[i])
+     // END EDIT
 }
 
 
@@ -73,8 +106,8 @@ ghost predicate Safety(v:Variables) {
 ghost predicate ClientHoldsLock(v: Variables, clientIndex: nat)
   requires v.WellFormed()
 {
-  // FIXME: fill in here (solution: 1 line)
-   false  // Replace me
+  // DONE: fill in here (solution: 1 line)
+  clientIndex < v.numClients && v.clientHolds[clientIndex]
   // END EDIT
 }
 
@@ -91,6 +124,14 @@ lemma PseudoLiveness(clientA:nat, clientB:nat) returns (behavior:seq<Variables>)
   ensures ClientHoldsLock(behavior[1], clientA) // first clientA acquires lock
   ensures ClientHoldsLock(behavior[|behavior|-1], clientB) // eventually clientB acquires lock
 {
-  // FIXME: fill in here (solution: 9 lines)
+  // DONE: fill in here (solution: 9 lines)
+  var state0 := Variables(3, true, seq(3, i => false), seq(3, i => false));
+  var state1 := Variables(3, false, seq(3, i => i == clientA), seq(3, i => i == clientA));
+  var state2 := Variables(3, true, seq(3, i => false), seq(3, i => false));
+  var state3 := Variables(3, false, seq(3, i => i == clientB), seq(3, i => i == clientB));
+  behavior := [state0, state1, state2, state3];
+  assert NextStep(state0, state1, AcquireLockStep(clientA));
+  assert NextStep(state1, state2, ReleaseLockStep(clientA));
+  assert NextStep(state2, state3, AcquireLockStep(clientB));
   // END EDIT
 }
